correctness statements cleaned

c/poc/strlen_spec.v
@@ -87,13 +87,6 @@ Definition VintN:= fun n => Vint (Int.repr(Z_of_nat n)).
 Notation gso := PTree.gso.
 Notation gss := PTree.gss.
 
-(* TODO : fix this *)
-Inductive C_string (m : Mem.mem) (b : block) (ofs : Z) (len : nat) :=
-  is_C_string : forall n i, (0 < Z.of_nat n < Int.modulus) ->
-                        (0 <= i < len)%nat ->
-                        Mem.load Mint8signed m b (ofs + Z_of_nat i) = Some (VintN n) ->
-                        Mem.load Mint8signed m b (ofs + Z_of_nat len) = Some (VintZ 0) ->
-                        C_string m b ofs len.
 
 (* Semantics of a C light function: *)
 
@@ -304,31 +297,81 @@ Proof.
 Admitted.
 
 
-Lemma strlen_correct : Archi.ptr64 = false -> forall ge e m b ofs le len,
+(* On a string of length 2 C light function evaluates to 0 *)
+Lemma strlen_correct_test1 :
+  (* with this assumption Ptrofs.modulus = Int.modulus, ptherwise Ptrofs.modulus > Int.modulus *)
+  Archi.ptr64 = false ->
+  forall ge e m b ofs le len,                       
+    (* Preconditions on the length of the string and valid offset *)
+    0 < ofs < Ptrofs.modulus ->
+    Z_of_nat len < Int.modulus ->
+    ofs + Z_of_nat len < Ptrofs.modulus ->                      
+    (* Initialize local variables *)
+    le!_input = Some (Vptr b (Ptrofs.repr ofs)) ->
+    le!_output = Some (VintZ 0) ->                     
+    (* Precondition: reading  C string of length 2 from memory *)
+    (exists z0, 0 < z0 /\ Mem.load Mint8signed m b ofs = Some (VintZ 1)) ->
+    (exists z1, 0 < z1 /\ Mem.load Mint8signed m b (ofs + 1) = Some (VintZ 1))  ->
+    Mem.load Mint8signed m b (ofs + 2) = Some (VintZ 0)  ->
+    (* C light expression f_strlen returns O and assigns O to output variable *)
+    exists t le', exec_stmt ge e le m f_strlen.(fn_body) t le' m (Out_return (Some ((VintZ 2),tuint))) /\ (le'!_output) = Some (VintZ 2).
+Proof.
+  intros.
+  destruct H5. destruct H5.
+  destruct H6. destruct H6.
+  repeat eexists. 
+  - seq1.
+    + seq1.
+      * sset. (* evaluate expression *) repeat econstructor.
+      * (* loop 1 *)
+        loop. repeat econstructor. repeat gso_assumption. eapply gss.        repeat econstructor. simpl. replace (Ptrofs.unsigned
+                                               (Ptrofs.add (Ptrofs.repr ofs) (Ptrofs.mul (Ptrofs.repr 1) (Ptrofs.of_intu (Int.repr 0))))) with ofs. apply H8.  { pose (Ptrofs.modulus_eq32 H). ptrofs_compute_add_mul. all: nia. } repeat econstructor. simpl. repeat econstructor. econstructor. repeat econstructor. repeat econstructor. apply gss. repeat econstructor.
+
+        (* loop 2 *)
+        loop. repeat econstructor. rewrite gso; repeat gso_assumption. eapply gss.
+        repeat econstructor. simpl. replace (Ptrofs.unsigned
+       (Ptrofs.add (Ptrofs.repr ofs)
+                   (Ptrofs.mul (Ptrofs.repr 1) (Ptrofs.of_intu (Int.add (Int.repr 0) (Int.repr 1)))))) with (ofs + 1). apply H9.  { pose (Ptrofs.modulus_eq32 H). ptrofs_compute_add_mul. all: admit. }        repeat econstructor. simpl. repeat econstructor. econstructor. repeat econstructor. repeat econstructor. apply gss. repeat econstructor.
+         (* exit loop *)
+        eapply exec_Sloop_stop1. (* break from the loop *)
+        repeat econstructor.  rewrite gso; repeat gso_assumption.  rewrite gso; repeat gso_assumption.  eapply gss.
+        repeat econstructor. simpl.
+        replace  (Ptrofs.unsigned
+       (Ptrofs.add (Ptrofs.repr ofs)
+          (Ptrofs.mul (Ptrofs.repr 1)
+             (Ptrofs.of_intu (Int.add (Int.add (Int.repr 0) (Int.repr 1)) (Int.repr 1)))))) with (ofs + 2). apply H7. { admit. }
+        repeat econstructor. simpl. repeat econstructor. econstructor. econstructor.
+    + (* return statement *)
+      repeat econstructor. eapply gss.
+  - eapply gss.
+Admitted.
+
+Lemma strlen_loop_continue_correct : Archi.ptr64 = false -> forall ge e m b ofs outp le,
       
-      (0 <= Z_of_nat len < Int.modulus ) -> (* len is within bounds *)
-      0 < ofs < Ptrofs.modulus -> 
-      (ofs + Z_of_nat len) < Ptrofs.modulus ->  (* the offsets are valid *)
-  
-      le!_input = Some (Vptr b (Ptrofs.repr ofs)) -> (* input is an address [b,ofs] *) 
-      le!_output = Some (VintZ 0) -> (* we start from 0 *)
+      1 <= Z.of_nat (S outp) < Ptrofs.modulus ->
+      ofs + Z.of_nat (S outp) < Ptrofs.modulus ->
+      0 < ofs < Ptrofs.modulus ->
+      0 <= Z.of_nat outp < Ptrofs.modulus ->
       
-      C_string m b ofs len -> (* [b,ofs] points to a string of length len in memory m *)
+      le!_input = Some (Vptr b (Ptrofs.repr (ofs + (Z.of_nat outp)))) ->
+      le!_output = Some (VintN outp) ->
       
-      exists t le', exec_stmt ge e le m f_strlen_loop t le' m (Out_return (Some (VintN len, tuint))) /\
-               (le'!_output) = Some (VintN len).
-(* the C light expression evaluates to outcome Out_return (Some VintN len) and output is set to len *)
+      (exists z, 0 < z < Int.modulus /\
+Mem.load Mint8signed m b (ofs + (Z_of_nat outp)) = Some (Vint (Int.repr z))) ->
+      
+      exists t le', exec_stmt ge e le m f_strlen_loop t le' m Out_normal /\ (le'!_output) = Some (VintN (S outp)).
 Admitted.
 
 
-Lemma strlen_corr2 : (* with this assumption Ptrofs.modulus = Int.modulus, ptherwise Ptrofs.modulus > Int.modulus *)
+Lemma strlen_correct : (* with this assumption Ptrofs.modulus = Int.modulus, ptherwise Ptrofs.modulus > Int.modulus *)
   Archi.ptr64 = false ->
   forall ge e m b ofs le len,
                        
-               (* Preconditions on the length of the string and valid offset *)
+    (* Preconditions on the length of the string and valid offset *)
+    (* 0 < Z.of_nat z < Int.modulus -> *) 
     0 < ofs < Ptrofs.modulus ->
-    Z_of_nat len < Int.modulus ->
-    ofs + Z_of_nat len < Ptrofs.modulus ->
+    Z_of_nat (S len) < Int.modulus ->
+    ofs + Z_of_nat (S len) < Ptrofs.modulus ->
                        
                        (* Initialize local variables *)
     le!_input = Some (Vptr b (Ptrofs.repr ofs)) ->
@@ -336,83 +379,38 @@ Lemma strlen_corr2 : (* with this assumption Ptrofs.modulus = Int.modulus, pther
 
                        
        (* Precondition: reading C string from memory *)
-    forall i z, (i < len)%nat ->
-           Mem.load chunk m b (ofs + Z.of_nat i) = Some (VintN (S z)) ->
-           Mem.load chunk m b ofs = Some (VintN O) ->
+    forall i, (i < len)%nat ->
+           (exists z, 0 < z /\ Mem.load chunk m b (ofs + Z.of_nat i) = Some (VintZ z)) ->
+           Mem.load chunk m b (ofs + Z.of_nat len) = Some (VintN O) ->
            
       exists t le', exec_stmt ge e le m f_strlen.(fn_body) t le' m (Out_return (Some ((VintN len),tuint))) /\
                     (le'!_output) = Some (VintN len).
 Proof.
   induction len.
-  - (* Base case *) intro L. intros.
-    apply (strlen_loop_break_correct H _  _ _ b ofs _ _).
-    (* 1,2,3: nia. *)    
-     all: try nia ; try assumption. inversion H3. simpl; unfold VintZ in H5; replace (ofs + 0) with ofs by lia. assumption. inversion H3. simpl; unfold VintZ in H5; replace (ofs + 0) with ofs by lia. assumption.
-  - (* Induction Step *) intro L. intros.
-    assert (C_string m b ofs len).
-    { inversion H3. admit. }
-    assert  (0 <= Z_of_nat len < Int.modulus ). { clear IHlen. lia. }
-    assert (ofs + Z.of_nat len < Ptrofs.modulus). { clear IHlen. nia. }                                   
-    pose (H8:= IHlen H7 H0 H1 H2 H5 H6).
-    destruct H8. destruct H8. destruct H8. clear IHlen.
-    assert  (exists t, exec_stmt ge e x0 m f_strlen_loop t (PTree.set _output (VintN (S len)) x0) m Out_normal /\ le ! _output = Some (Vint_of_nat (Datatypes.S len))).
-    { repeat eexists.
-      +  Print exec_stmt. eapply exec_Sloop_loop.
-         repeat econstructor. Admitted.
-
-Lemma strlen_loop_continue_correct : Archi.ptr64 = false -> forall z ge e m b ofs outp le,
-      
-      1 <= Z.of_nat (S outp) < Ptrofs.modulus ->
-      0 < z < Int.modulus ->
-      ofs + Z.of_nat ( S outp ) < Ptrofs.modulus ->
-      0 < ofs < Ptrofs.modulus ->
-      0 <= Z.of_nat outp < Ptrofs.modulus ->
-      
-      le!_input = Some (Vptr b (Ptrofs.repr ofs)) ->
-      le!_output = Some (VintN outp) ->
-      
-      Mem.load Mint8signed m b (ofs + (Z_of_nat outp)) = Some (Vint (Int.repr z)) ->
-      
-      exists t le', exec_stmt ge e le m f_strlen_loop t le' m Out_normal /\
-               (le'!_output) = Some (VintN (S outp)).
-Proof.
-  intros.
-  eexists.
-  exists (PTree.set _output (VintN (S outp)) le).
-  split.
-  + Print exec_stmt. eapply exec_Sloop_loop. repeat econstructor. apply H5. apply H6.
-    econstructor. simpl. replace  (Ptrofs.unsigned
-       (Ptrofs.add (Ptrofs.repr ofs)
-                   (Ptrofs.mul (Ptrofs.repr 1) (Ptrofs.of_intu (Int.repr (Z.of_nat outp)))))) with (ofs + Z.of_nat outp). apply H7. { pose (Ptrofs.modulus_eq32 H). rewrite Ptrofs.mul_commut. rewrite Ptrofs.mul_one. ptrofs_compute_add_mul. all: nia. }
-   econstructor. simpl. replace  (negb (Int.eq (Int.repr z) (Int.repr 0))) with true.
-    econstructor.  admit.
-    repeat econstructor.  econstructor.
-    repeat econstructor. apply H6.
-    repeat econstructor.
-    assert (exists t, exec_stmt ge e (PTree.set _output (Vint (Int.add (Int.repr (Z.of_nat outp)) (Int.repr 1))) le)
-    m
-    (Sloop
-       (Sifthenelse
-          (Ebinop One
-             (Ederef
-                (Ebinop Oadd (Etempvar _input (tptr tschar)) (Etempvar _output tuint)
-                   (tptr tschar)) tschar) (Econst_int (Int.repr 0) tint) tint) Sskip Sbreak)
-       (Sset _output (Ebinop Oadd (Etempvar _output tuint) (Econst_int (Int.repr 1) tint) tuint)))
-    t (PTree.set _output (Vint (Int.add (Int.repr (Z.of_nat outp)) (Int.repr 1))) le) m Out_normal ).
-    
-    fold f_strlen_loop. apply (strlen_loop_break_correct2 H _  _ _ b ofs (S outp) _) ; try nia ; try assumption. rewrite PTree.gso. assumption. cbv. congruence.    
-
-    replace (Vint (Int.add (Int.repr (Z.of_nat outp)) (Int.repr 1))) with  (VintN (S outp)).
-    apply PTree.gss.
-    { unfold VintN. f_equal. unfold Int.add. ints_to_Z. f_equal. nia. nia. admit.
-    (* from H0 *) }
-    admit.
-    replace (VintN (S outp)) with  (Vint (Int.add (Int.repr (Z.of_nat outp)) (Int.repr 1))).
-    edestruct H8.
-    admit.
-    admit.
-Admitted.
   
+  (* Base case *)
+ - intros. destruct H6. destruct H6. omega.
+ 
+  (* Inductive Step *)
+ - (* assert (exists t le', exec_stmt ge e le m f_strlen_loop t le' m Out_normal /\
+                    le' ! _output = Some (VintN len)).
+   { admit. } *)
+   intros.  destruct H6. destruct H6.
+   induction i.
+   -- repeat eexists.
+     (* Base case *) 
+      --- seq1.
+         + seq1.
+           * sset. repeat econstructor.
+           * fold f_strlen_loop.  pose (I := strlen_loop_break_correct2 H ge e m b ofs (S len)).
+            (*  assert ( exists t, exec_stmt ge e (PTree.set _output (VintN (S len)) le) m
+                                     f_strlen_loop t (PTree.set _output (VintN (S len)) le) m Out_normal). eapply I. 1,2,3: nia. gso_assumption. assumption. gso_assumption. apply gss. assumption.  ; try assumption. cbv. congruence.
+   --  (* Inductive Step *) intros. eapply IHz.
+   { admit. (* H0 *) } 1,2,3: nia. 
+   1,2: gso_assumption. apply H6. 
+   replace ofs with (ofs + Z.of_nat 0) by lia ; assumption. *)
+Admitted. 
+                        
 (* Old stuff: One direction of correctness, using functional spec, below relational with proof attempt *)
 
  Definition strlen_C_fun_corr_r :
