c/poc/sandbox.v
@@ -1,0 +1,139 @@
+Lemma strlen_loop_continue_correct : Archi.ptr64 = false -> forall z ge e m b ofs outp le,
+      
+      1 <= Z.of_nat (S outp) < Ptrofs.modulus ->
+      0 < z < Int.modulus ->
+      ofs + Z.of_nat ( S outp ) < Ptrofs.modulus ->
+      0 < ofs < Ptrofs.modulus ->
+      0 <= Z.of_nat outp < Ptrofs.modulus ->
+      
+      le!_input = Some (Vptr b (Ptrofs.repr (ofs + (Z.of_nat outp)))) ->
+      le!_output = Some (VintN outp) ->
+      
+      Mem.load Mint8signed m b (ofs + (Z_of_nat outp)) = Some (Vint (Int.repr z)) ->
+      
+      exists t le', exec_stmt ge e le m f_strlen_loop t le' m Out_normal /\ (le'!_output) = Some (VintN (S outp)).
+Proof.
+  induction outp.
+  intros.
+  repeat eexists.
+  - loop.  repeat econstructor; repeat gso_assumption. repeat econstructor. simpl.
+     replace  (Ptrofs.unsigned
+       (Ptrofs.add (Ptrofs.repr (ofs + 0))
+                   (Ptrofs.mul (Ptrofs.repr 1) (Ptrofs.of_intu (Int.repr 0))))) with (ofs + Z.of_nat 0). apply H7. { pose (Ptrofs.modulus_eq32 H). rewrite Ptrofs.mul_commut. rewrite Ptrofs.mul_one. ptrofs_compute_add_mul. all: nia. }
+   econstructor. simpl. replace  (negb (Int.eq (Int.repr z) (Int.repr 0))) with true.
+    econstructor. { admit. } 
+    repeat econstructor. econstructor.
+    repeat econstructor. gso_assumption.
+    repeat econstructor.
+    assert (exists t, exec_stmt ge e (PTree.set _output (Vint (Int.add (Int.repr (Z.of_nat 0)) (Int.repr 1))) le)
+    m
+    (Sloop
+       (Sifthenelse
+          (Ebinop One
+             (Ederef
+                (Ebinop Oadd (Etempvar _input (tptr tschar)) (Etempvar _output tuint)
+                   (tptr tschar)) tschar) (Econst_int (Int.repr 0) tint) tint) Sskip Sbreak)
+       (Sset _output (Ebinop Oadd (Etempvar _output tuint) (Econst_int (Int.repr 1) tint) tuint)))
+    t (PTree.set _output (Vint (Int.add (Int.repr (Z.of_nat 0)) (Int.repr 1))) le) m Out_normal ).
+    
+    fold f_strlen_loop. apply (strlen_loop_break_correct2 H _  _ _ b ofs (S O) _) ; try nia ; try assumption.  gso_assumption.
+  admit. admit. apply gss.
+Admitted.
+
+
+Lemma strlen_non_empty_corr : (* with this assumption Ptrofs.modulus = Int.modulus, ptherwise Ptrofs.modulus > Int.modulus *)
+  Archi.ptr64 = false ->
+  forall ge e m b ofs le len,
+                       
+               (* Preconditions on the length of the string and valid offset *)
+    0 < ofs < Ptrofs.modulus ->
+    Z_of_nat (S len) < Int.modulus ->
+    ofs + Z_of_nat (S len) < Ptrofs.modulus ->
+                       
+                       (* Initialize local variables *)
+    le!_input = Some (Vptr b (Ptrofs.repr ofs)) ->
+    le!_output = Some (VintZ 0) ->
+
+                       
+       (* Precondition: reading C string from memory *)
+    forall i z, (i < S len)%nat ->
+           Mem.load chunk m b (ofs + Z.of_nat i) = Some (VintN (S z)) ->
+           Mem.load chunk m b (ofs + Z.of_nat (S len)) = Some (VintN O) ->
+           
+      exists t le', exec_stmt ge e le m f_strlen.(fn_body) t le' m (Out_return (Some ((VintN (S len)),tuint))) /\
+                    (le'!_output) = Some (VintN (S len)).
+Proof.
+  induction len.
+  - (* Base case *) intro L. intros.
+     repeat eexists.
+ 
+  -- seq1.
+    + seq1.
+      * sset. (* evaluate expression *) repeat econstructor.
+      * (* loop 1 *)
+        loop. repeat econstructor. repeat gso_assumption. eapply gss.        repeat econstructor. simpl. replace (Ptrofs.unsigned
+                                               (Ptrofs.add (Ptrofs.repr ofs) (Ptrofs.mul (Ptrofs.repr 1) (Ptrofs.of_intu (Int.repr 0))))) with ofs. assert (i = O). omega. rewrite H7 in H5. simpl in H5. replace (ofs) with (ofs + 0) by lia. apply H5.  { pose (Ptrofs.modulus_eq32 H). ptrofs_compute_add_mul. all: nia. } repeat econstructor. simpl. replace  (negb
+          (Int.eq (Int.repr (Z.pos (Pos.of_succ_nat z)))
+                  (Int.repr 0))) with true.  repeat econstructor. { admit.  } econstructor. repeat econstructor. repeat econstructor. apply gss. repeat econstructor.
+
+        (* exit loop *)
+        eapply exec_Sloop_stop1. (* break from the loop *)
+        repeat econstructor.  rewrite gso; repeat gso_assumption.  eapply gss.
+        repeat econstructor. simpl.
+        replace (Ptrofs.unsigned
+       (Ptrofs.add (Ptrofs.repr ofs)
+                   (Ptrofs.mul (Ptrofs.repr 1) (Ptrofs.of_intu (Int.add (Int.repr 0) (Int.repr 1)))))) with (ofs + 1). apply H6.  { pose (Ptrofs.modulus_eq32 H). ptrofs_compute_add_mul. all: admit. }
+                                                                                                                                  repeat econstructor. simpl. repeat econstructor. econstructor. econstructor.
+    + (* return statement *)
+      repeat econstructor. eapply gss.
+      -- eapply gss.
+
+   -. intros. repeat eexists. -- seq1.
+    + seq1.
+      * sset. (* evaluate expression *) repeat econstructor.
+      * (* loop 1 *)
+        loop. repeat econstructor. repeat gso_assumption. eapply gss.        repeat econstructor. simpl.
+        induction i.
+        replace (Ptrofs.unsigned
+                                               (Ptrofs.add (Ptrofs.repr ofs) (Ptrofs.mul (Ptrofs.repr 1) (Ptrofs.of_intu (Int.repr 0))))) with ofs. simpl in H6. replace ofs with  (ofs + 0) by lia. apply H6. { admit. } apply IHi. omega.
+                                                                                                                                  
+    apply (strlen_loop_break_correct H _  _ _ b ofs _ _).
+    (* 1,2,3: nia. *)    
+     all: try nia ; try assumption. inversion H3. simpl; unfold VintZ in H5; replace (ofs + 0) with ofs by lia. assumption. inversion H3. simpl; unfold VintZ in H5; replace (ofs + 0) with ofs by lia. assumption.
+  - (* Induction Step *) intro L. intros.
+    assert (C_string m b ofs len).
+    { inversion H3. admit. }
+    assert  (0 <= Z_of_nat len < Int.modulus ). { clear IHlen. lia. }
+    assert (ofs + Z.of_nat len < Ptrofs.modulus). { clear IHlen. nia. }                                   
+    pose (H8:= IHlen H7 H0 H1 H2 H5 H6).
+    destruct H8. destruct H8. destruct H8. clear IHlen.
+    assert  (exists t, exec_stmt ge e x0 m f_strlen_loop t (PTree.set _output (VintN (S len)) x0) m Out_normal /\ le ! _output = Some (Vint_of_nat (Datatypes.S len))).
+    { repeat eexists.
+      +  Print exec_stmt. eapply exec_Sloop_loop.
+         repeat econstructor. Admitted.
+
+
+(* TODO : fix this *)
+Inductive C_string (m : Mem.mem) (b : block) (ofs : Z) (len : nat) :=
+  is_C_string : forall n i, (0 < Z.of_nat n < Int.modulus) ->
+                        (0 <= i < len)%nat ->
+                        Mem.load Mint8signed m b (ofs + Z_of_nat i) = Some (VintN n) ->
+                        Mem.load Mint8signed m b (ofs + Z_of_nat len) = Some (VintZ 0) ->
+                        C_string m b ofs len.
+
+
+Lemma strlen_correct_with_C_string : Archi.ptr64 = false -> forall ge e m b ofs le len,
+      
+      (0 <= Z_of_nat len < Int.modulus ) -> (* len is within bounds *)
+      0 < ofs < Ptrofs.modulus -> 
+      (ofs + Z_of_nat len) < Ptrofs.modulus ->  (* the offsets are valid *)
+  
+      le!_input = Some (Vptr b (Ptrofs.repr ofs)) -> (* input is an address [b,ofs] *) 
+      le!_output = Some (VintZ 0) -> (* we start from 0 *)
+      
+      C_string m b ofs len -> (* [b,ofs] points to a string of length len in memory m *)
+      
+      exists t le', exec_stmt ge e le m f_strlen_loop t le' m (Out_return (Some (VintN len, tuint))) /\
+               (le'!_output) = Some (VintN len).
+(* the C light expression evaluates to outcome Out_return (Some VintN len) and output is set to len *)
+Admitted.
